src3.0/Vellvm/Dominators/dom_list_tree.v
@@ -4,40 +4,8 @@ Require Import syntax.
 Require Import infrastructure_props.
 Require Import Metatheory.
 Require Import Program.Tactics.
+Require Import dom_tree.
 Require Import push_iter.
-
-Inductive DTree : Set :=
-| DT_node : positive -> DTrees -> DTree
-with DTrees : Set :=
-| DT_nil : DTrees
-| DT_cons : DTree -> DTrees -> DTrees
-.
-
-Fixpoint list2tree hd tl := 
-match tl with
-| nil => DT_node hd DT_nil
-| hd'::tl' => DT_node hd (DT_cons (list2tree hd' tl') DT_nil)
-end.
-
-Fixpoint dtree_insert dt parent child tl : DTree :=
-match dt with
-| DT_node l0 dts0 =>
-    if positive_eq_dec parent l0
-    then DT_node l0 (dtrees_insert dts0 child tl)
-    else dt
-end
-with dtrees_insert (dts: DTrees) child tl : DTrees :=
-match dts with
-| DT_nil => DT_cons (list2tree child tl) DT_nil
-| DT_cons dt0 dts0 =>
-    let '(DT_node l0 _) := dt0 in
-    if positive_eq_dec l0 child then 
-      match tl with
-      | child'::tl' => DT_cons (dtree_insert dt0 child child' tl') dts0
-      | _ => dts
-      end
-    else DT_cons dt0 (dtrees_insert dts0 child tl)
-end.
 
 Fixpoint compute_sdom_chains_aux (res: positive -> LDoms.t)
   (bd: list positive) (acc: list (positive * list positive)) 
@@ -56,448 +24,33 @@ Definition compute_sdom_chains (res: positive -> LDoms.t) rd
   : list (positive * list positive) :=
 compute_sdom_chains_aux res rd nil.
 
-Definition create_dtree_from_chain dt chain : DTree :=
-match chain with
-| p::(ch::chain') => dtree_insert dt p ch chain'
-| _ => dt
-end.
-
 Definition create_dtree (pe:positive) (rd:list positive) 
   (res: positive -> LDoms.t) : DTree :=
 let chains := compute_sdom_chains res rd in
 fold_left 
-  (fun acc elt => let '(_, chain):=elt in create_dtree_from_chain acc chain)
+  (fun acc elt => 
+   let '(_, chain):=elt in create_dtree_from_chain positive_eq_dec acc chain)
   chains (DT_node pe DT_nil).
-
-Fixpoint in_children_roots child dts : bool :=
-match dts with
-| DT_nil => false
-| DT_cons (DT_node l0 _) dts' =>
-    if (positive_eq_dec l0 child) then true else in_children_roots child dts'
-end.
-
-Fixpoint is_dtree_edge dt parent child : bool :=
-match dt with
-| DT_node l0 dts0 =>
-    if (positive_eq_dec parent l0) then
-      if in_children_roots child dts0 then true
-      else is_dtrees_edge dts0 parent child
-    else is_dtrees_edge dts0 parent child
-end
-with is_dtrees_edge (dts: DTrees) parent child : bool :=
-match dts with
-| DT_nil => false
-| DT_cons dt0 dts0 =>
-    is_dtree_edge dt0 parent child || is_dtrees_edge dts0 parent child
-end.
-
-Scheme dtree_rec2 := Induction for DTree Sort Set
-  with dtrees_rec2 := Induction for DTrees Sort Set.
-
-Definition dtree_mutrec P P' :=
-  fun h1 h2 h3 =>
-    (pair (@dtree_rec2 P P' h1 h2 h3) (@dtrees_rec2 P P' h1 h2 h3)).
-
-Fixpoint is_chain_edge (chain:list positive) p0 ch0 : Prop :=
-match chain with
-| p::((ch::_) as chain') => (p = p0 /\ ch = ch0) \/ is_chain_edge chain' p0 ch0
-| _ => False
-end.
-
-Lemma dtrees_insert__in_children_roots: forall ch ch0 tl dts
-  (Hin: in_children_roots ch dts = true),
-  in_children_roots ch (dtrees_insert dts ch0 tl) = true.
-Proof.
-  induction dts as [|[]]; simpl; intro; try congruence.
-    destruct_if.
-      destruct_if.
-        destruct tl; simpl.
-          destruct_if.
-          destruct_if. destruct_if.
-        simpl. destruct_if.
-      destruct_if.
-        destruct tl; simpl.
-          destruct_if.
-          destruct_if; try congruence.
-            destruct_if.
-        simpl. 
-        destruct_if.
-          rewrite IHdts; auto.
-Qed.
-
-Lemma list2tree_spec: forall ch0 tl,
-  exists dts, list2tree ch0 tl = DT_node ch0 dts.
-Proof.
-  destruct tl; simpl; eauto.
-Qed.
-
-Lemma inserted_in_children_roots: forall ch ch0 tl dts
-  (Hnotin: in_children_roots ch dts = false)
-  (Hin: in_children_roots ch (dtrees_insert dts ch0 tl) = true),
-  ch = ch0.
-Proof.
-  induction dts as [|[]]; simpl; intros.
-  Case "1".
-    destruct (list2tree_spec ch0 tl) as [dts Heq].
-    rewrite Heq in Hin.
-    destruct_if; try solve [auto | congruence].
-  Case "2".
-    destruct_if.
-    SCase "2.1".
-      destruct_if; try congruence.
-      destruct_if.
-      destruct tl; simpl in *.
-        destruct_if; try congruence.
-        destruct_if; try congruence.
-    SCase "2.2".
-      destruct_if; try solve [congruence | auto].
-Qed.
-
-Lemma inserted_in_children_roots': forall ch0 tl dts,
-  in_children_roots ch0 (dtrees_insert dts ch0 tl) = true.
-Proof.
-  induction dts as [|[]]; simpl; intros.
-  Case "1".
-    destruct (list2tree_spec ch0 tl) as [dts Heq].
-    rewrite Heq.
-    destruct_if; try solve [auto | congruence].
-  Case "2".
-    destruct_if.
-    SCase "2.1".
-      destruct_if; try congruence.
-      destruct tl; simpl in *.
-        destruct_if; try congruence.
-        destruct_if; try congruence.
-    SCase "2.2".
-      simpl. destruct_if; try solve [congruence | auto].
-Qed.
-
-Definition get_dtree_root (dt:DTree) : positive :=
-match dt with
-| DT_node l0 _ => l0
-end.
-
-Definition dtree_insert__is_dtree_edge_prop (dt:DTree) :=
-forall p ch tl p0 ch0,
-  is_dtree_edge (dtree_insert dt p ch tl) p0 ch0 = true <->
-  is_dtree_edge dt p0 ch0 = true \/ 
-    (p = get_dtree_root dt /\ is_chain_edge (p::ch::tl) p0 ch0).
-
-Definition dtrees_insert__is_dtrees_edge_prop (dts:DTrees) :=
-forall ch tl p0 ch0,
-  is_dtrees_edge (dtrees_insert dts ch tl) p0 ch0 = true <->
-  is_dtrees_edge dts p0 ch0 = true \/ is_chain_edge (ch::tl) p0 ch0.
-
-Lemma is_dtrees_egde_cons_elim: forall dt1 dts2 p ch
-  (Hin: is_dtrees_edge (DT_cons dt1 dts2) p ch = true),
-  is_dtree_edge dt1 p ch = true \/ is_dtrees_edge dts2 p ch = true.
-Proof.
-  simpl.
-  intros.
-  binvt Hin as J1 J2; auto.
-Qed.
-
-Lemma is_dtrees_egde_cons_intro: forall dt1 dts2 p ch
-  (Hin: is_dtree_edge dt1 p ch = true \/ is_dtrees_edge dts2 p ch = true),
-  is_dtrees_edge (DT_cons dt1 dts2) p ch = true.
-Proof.
-  simpl.
-  intros. auto with datatypes v62.
-Qed.
-
-Lemma DT_nil_has_no_dtree_edges: forall p ch,
-  is_dtrees_edge DT_nil p ch = false.
-Proof. simpl. auto. Qed.
-
-Lemma single_node_has_no_dtree_edges: forall hd p ch,
-  is_dtree_edge (DT_node hd DT_nil) p ch = false.
-Proof. intros. simpl. destruct_if. Qed.
-
-Lemma is_dtree_edge_of_list2tree__is_chain_edge: forall p0 ch0 tl ch
-  (Hin: is_dtree_edge (list2tree ch tl) p0 ch0 = true),
-  is_chain_edge (ch::tl) p0 ch0.
-Proof.
-Local Opaque is_dtrees_edge.
-  induction tl as [|hd tl']; simpl; intros.
-    destruct_if; congruence.
-
-    destruct_if.
-      destruct (list2tree_spec hd tl') as [x Heq].
-      rewrite Heq in H0.
-      destruct (positive_eq_dec hd ch0); subst; auto.
-        apply is_dtrees_egde_cons_elim in H0.
-        destruct H0 as [H0 | H0].
-          right. apply IHtl'. rewrite Heq. auto.
-
-          rewrite DT_nil_has_no_dtree_edges in H0. congruence.
-       apply is_dtrees_egde_cons_elim in H0.
-       destruct H0 as [H0 | H0].
-         right. apply IHtl'. auto.
-         rewrite DT_nil_has_no_dtree_edges in H0. congruence.
-Qed.
-
-Lemma is_chain_edge__is_dtree_edge_of_list2tree: forall p0 ch0 tl ch
-  (Hin: is_chain_edge (ch::tl) p0 ch0),
-  is_dtree_edge (list2tree ch tl) p0 ch0 = true.
-Proof.
-  induction tl as [|hd tl']; simpl; intros.
-    tauto.
-
-    destruct (list2tree_spec hd tl') as [x Heq].
-    rewrite Heq.
-    destruct Hin as [[EQ1 EQ2] | Hin]; subst.
-      destruct_if.
-      destruct (positive_eq_dec ch0 ch0); try congruence.
-
-      destruct (positive_eq_dec p0 ch); subst.
-        destruct (positive_eq_dec hd ch0); subst; auto.
-          apply is_dtrees_egde_cons_intro.
-          left. rewrite <- Heq. apply IHtl'; auto.          
-
-        apply is_dtrees_egde_cons_intro.
-        left. rewrite <- Heq. apply IHtl'; auto.          
-Transparent is_dtrees_edge.
-Qed.
-
-Lemma dtree_insert__is_dtree_edge_mutrec :
-  (forall dt, dtree_insert__is_dtree_edge_prop dt) *
-  (forall dts, dtrees_insert__is_dtrees_edge_prop dts).
-Proof.
-  apply dtree_mutrec;
-    unfold dtree_insert__is_dtree_edge_prop, dtrees_insert__is_dtrees_edge_prop;
-    intros; simpl.
-  Case "DT_node".
-    destruct_if.
-    SCase "p0 = root".
-      destruct_if.
-      SSCase "p1 = root".
-        remember (in_children_roots ch0 d) as R.
-        destruct R; simpl.
-        SSSCase "ch0 in d".
-          destruct_if; try congruence.
-          split; intro J; auto.
-            rewrite dtrees_insert__in_children_roots; auto.
-
-        SSSCase "ch0 notin d".
-          destruct_if; try congruence.
-          remember (in_children_roots ch0 (dtrees_insert d ch tl)) as R.
-          destruct R; simpl.
-          SSSSCase "ch0 in inserted".
-            split; intro; auto.
-              right.
-              split; auto.
-                left.
-                split; auto.
-                  symmetry in HeqR3.
-                  eapply inserted_in_children_roots in HeqR3; eauto.
-          SSSSCase "ch0 notin inserted".
-            split; intro J.
-            SSSSSCase "1".
-              apply H in J.
-              destruct J as [J | J]; auto.
-            SSSSSCase "2".
-              apply H. 
-              destruct J as [J | [J1 [[EQ1 EQ2] |J2]]]; subst; auto.
-                rewrite inserted_in_children_roots' in HeqR3. congruence.
-      SSCase "p1 <> root".
-        simpl.
-        destruct_if; try congruence.
-        split; intro J.
-          SSSCase "1".
-            apply H in J.
-            destruct J as [J | J]; auto.
-          SSSCase "2".
-            apply H. 
-            destruct J as [J | [J1 [[EQ1 EQ2] |J2]]]; subst; auto.
-    SCase "p0 <> root".
-      simpl.
-      destruct_if.
-      SSCase "p1 = root".
-        split; intro J; auto.
-          SSSCase "1".
-          remember (in_children_roots ch0 d) as R.
-          destruct R; simpl; auto.
-            destruct J as [J | [J1 [[EQ1 EQ2] |J2]]]; subst; auto.
-      SSCase "p1 <> root".
-        split; intro J; auto.
-          destruct J as [J | [J1 [[EQ1 EQ2] |J2]]]; subst; auto.
-
-  Case "DT_nil".
-    split; intros J.
-      bdestruct J as J1 J2; try congruence.
-        right.
-        apply is_dtree_edge_of_list2tree__is_chain_edge; auto.
-     destruct J as [J | J]; try congruence.
-
-      rewrite is_chain_edge__is_dtree_edge_of_list2tree; auto.
-
-  Case "DT_cons".
-    destruct d as [l0 ?].
-    destruct_if.
-    SCase "l0 = ch".
-      destruct tl; try tauto.
-      SSCase "tl<>nil".
-        split; intro J.
-        SSSCase "1".
-          apply is_dtrees_egde_cons_elim in J.
-          destruct J as [J | J].
-          SSSSCase "1.1".
-            apply H in J. 
-            destruct J as [J1 |[J2 J3]]; auto.
-              rewrite J1. auto.
-          SSSSCase "1.2".
-            left. rewrite J. auto with datatypes v62.
-        SSSCase "2".
-          apply is_dtrees_egde_cons_intro.
-          destruct J as [J | [[J1 J2] | J]]; subst.
-          SSSSCase "2.1".
-            binvt J as J1 J2; auto.
-              left. apply H; auto.
-          SSSSCase "2.2".
-            left. apply H; simpl; auto.
-          SSSSCase "2.3".
-            left. apply H; simpl; auto.
-    SCase "l0 <> ch".
-        split; intro J.
-        SSSCase "1".
-          apply is_dtrees_egde_cons_elim in J.
-          destruct J as [J | J].
-          SSSSCase "1.1".
-            left.
-            apply is_dtrees_egde_cons_intro; auto.
-          SSSSCase "1.2".
-            apply H0 in J.
-            destruct J as [J | J].
-              left. apply is_dtrees_egde_cons_intro; auto.
-              right. auto.
-        SSSCase "2".
-          apply is_dtrees_egde_cons_intro.
-          destruct J as [J | J].    
-          SSSSCase "2.1".
-            binvt J as J1 J2; auto.
-              right. apply H0; auto.
-          SSSSCase "2.2".
-            right. apply H0; auto.
-Qed.
-
-Lemma dtree_insert__is_dtree_edge : forall p ch tl p0 ch0 dt,
-  is_dtree_edge (dtree_insert dt p ch tl) p0 ch0 = true <->
-  is_dtree_edge dt p0 ch0 = true \/ 
-  p = get_dtree_root dt /\ is_chain_edge (p::ch::tl) p0 ch0.
-Proof.
-  destruct (dtree_insert__is_dtree_edge_mutrec).
-  unfold dtree_insert__is_dtree_edge_prop in *.
-  eauto.
-Qed.
-
-Definition chain_connects_dtree dt (chain:list positive) : Prop :=
-match chain with
-| entry :: _ :: _ => entry = get_dtree_root dt
-| _ => False
-end.
-
-Lemma create_dtree_from_chain__is_dtree_edge__is_chain_edge:
-  forall p0 ch0 chain dt,
-  (is_dtree_edge (create_dtree_from_chain dt chain) p0 ch0 = true ->
-   is_dtree_edge dt p0 ch0 = true \/ is_chain_edge chain p0 ch0) /\
-  (is_dtree_edge dt p0 ch0 = true \/
-   (chain_connects_dtree dt chain /\ is_chain_edge chain p0 ch0) ->
-   is_dtree_edge (create_dtree_from_chain dt chain) p0 ch0 = true).
-Proof.
-  intros.
-Local Opaque is_chain_edge.
-  destruct chain as [|p chain]; simpl; try tauto.
-  destruct chain as [|ch chain]; simpl; try tauto.
-  split; intros.
-    apply dtree_insert__is_dtree_edge in H. tauto.
-    apply dtree_insert__is_dtree_edge in H; auto.
-Transparent is_chain_edge.
-Qed.
-
-Lemma dtree_insert__get_dtree_root: forall dt p ch tl,
-  get_dtree_root dt = get_dtree_root (dtree_insert dt p ch tl).
-Proof.
-  destruct dt; simpl.
-  intros.
-  destruct_if; auto.
-Qed.
-
-Lemma create_dtree_from_chain__chain_connects_dtree: forall chain0 chain dt
-  (H: chain_connects_dtree dt chain0),
-  chain_connects_dtree (create_dtree_from_chain dt chain) chain0.
-Proof.
-  intros.
-  destruct chain0 as [|p0 chain0]; auto.
-  destruct chain0 as [|ch0 chain0]; auto.
-  simpl in *.
-  destruct chain as [|p chain]; auto.
-  destruct chain as [|ch chain]; auto.
-  subst. apply dtree_insert__get_dtree_root.
-Qed.
-
-Lemma fold_left_create_dtree_from_chain__is_dtree_edge__is_chain_edge:
-  forall p0 ch0 chains dt,
-  (is_dtree_edge
-    (fold_left
-      (fun (acc : DTree) (elt : positive * list positive) =>
-       let '(_, chain) := elt in create_dtree_from_chain acc chain)
-     chains dt) p0 ch0 = true ->
-  (is_dtree_edge dt p0 ch0 = true \/
-   exists l0, exists chain0,
-     List.In (l0, chain0) chains /\ is_chain_edge chain0 p0 ch0)) /\
-  ((is_dtree_edge dt p0 ch0 = true \/
-   exists l0, exists chain0,
-     List.In (l0, chain0) chains /\ chain_connects_dtree dt chain0 /\
-     is_chain_edge chain0 p0 ch0) ->
-   is_dtree_edge
-    (fold_left
-      (fun (acc : DTree) (elt : positive * list positive) =>
-       let '(_, chain) := elt in create_dtree_from_chain acc chain)
-     chains dt) p0 ch0 = true).
-Proof.
-  induction chains as [|[p l1] chains]; simpl; intros.
-    split; intro J; auto.
-      destruct J as [H | [l0 [chn0 [J1 J2]]]]; auto.
-
-    destruct (IHchains (create_dtree_from_chain dt l1)) as [J1 J2].
-    clear IHchains.
-    split; intros J.
-      apply J1 in J.
-      destruct J as [J | [l2 [chain2 [J3 J4]]]].
-        apply create_dtree_from_chain__is_dtree_edge__is_chain_edge in J.
-        destruct J as [J | J]; auto.
-          right. eauto. 
-        right. exists l2. exists chain2. auto.
-
-      apply J2.
-      destruct J as [J | [l2 [chain2 [J3 [J4 J5]]]]].
-        left.
-        apply create_dtree_from_chain__is_dtree_edge__is_chain_edge; auto.
-
-        destruct J3 as [J3 | J3].
-          inv J3. left.
-          apply create_dtree_from_chain__is_dtree_edge__is_chain_edge; auto.
-
-          right. exists l2. exists chain2. split; auto. split; auto.
-            apply create_dtree_from_chain__chain_connects_dtree; auto.
-Qed.
 
 Lemma create_dtree__wf_dtree_aux: forall pe rd res dt,
   create_dtree pe rd res = dt ->
   let chains := compute_sdom_chains res rd in
   forall p0 ch0,
-    (is_dtree_edge dt p0 ch0 = true ->
+    (is_dtree_edge positive_eq_dec dt p0 ch0 = true ->
       exists l0, exists chain0,
       List.In (l0, chain0) chains /\ is_chain_edge chain0 p0 ch0) /\
     ((exists l0, exists chain0,
       List.In (l0, chain0) chains /\
       chain_connects_dtree (DT_node pe DT_nil) chain0 /\
-     is_chain_edge chain0 p0 ch0) -> is_dtree_edge dt p0 ch0 = true).
+     is_chain_edge chain0 p0 ch0) -> 
+     is_dtree_edge positive_eq_dec dt p0 ch0 = true).
 Proof.
   unfold create_dtree.
   intros. subst.
-  destruct (@fold_left_create_dtree_from_chain__is_dtree_edge__is_chain_edge
-    p0 ch0 (compute_sdom_chains res rd) (DT_node pe DT_nil)) as [J1 J2].
+  destruct (fold_left_create_dtree_from_chain__is_dtree_edge__is_chain_edge
+    positive_eq_dec p0 ch0 (compute_sdom_chains res rd) 
+    (DT_node pe DT_nil)) 
+    as [J1 J2].
   split; intros J; auto.
     apply J1 in J.
     destruct J as [J | J]; auto.
@@ -563,66 +116,6 @@ Proof.
   apply compute_sdom_chains_aux_spec'; auto.
 Qed.
 
-Lemma is_chain_edge_tail: forall p0 ch0 ls2 ls1 
-  (Hintl: is_chain_edge ls2 p0 ch0),
-  is_chain_edge (ls1 ++ ls2) p0 ch0.
-Proof.
-  induction ls1; simpl; intros; auto.
-    case_eq (ls1 ++ ls2).
-      intro J.
-      apply app_eq_nil in J. 
-      destruct J; subst; simpl in Hintl; auto.
-
-      intros p l EQ.
-      rewrite <- EQ. auto.
-Qed.
-
-Lemma chain_edge_sorted: forall R p0 ch0 ls1 (Hedge: is_chain_edge ls1 p0 ch0)
-  (Hsort : Sorted R ls1), R p0 ch0.
-Proof.
-  induction 2; simpl in *.
-    tauto.
-
-    destruct l; try tauto.   
-    destruct Hedge as [[EQ1 EQ2] | Hedge]; subst; auto.
-      inv H. auto.
-Qed.
-
-Lemma is_chain_edge__inv: forall p0 ch0 l0 dts0
-  (Hedge: is_chain_edge (dts0 ++ [l0]) p0 ch0),
-  In p0 (dts0 ++ [l0]) /\ In ch0 (dts0 ++ [l0]) /\ dts0 <> nil.
-Proof.
-  induction dts0; simpl; intros.
-    tauto.
-
-    case_eq (dts0 ++ [l0]).
-      intro Heq.
-      destruct dts0; inv Heq.
-
-      intros p1 l1 Heq.
-      rewrite Heq in Hedge.
-      destruct Hedge as [[EQ1 EQ2] | Hedge]; subst.
-        simpl. 
-        split; auto.
-        split; auto.
-          congruence.
-
-        rewrite <- Heq in *.
-        apply IHdts0 in Hedge.
-        destruct Hedge as [J1 [J2 J3]].
-        split; auto.
-        split; auto.
-          congruence.     
-Qed.
-
-Lemma rev_non_nil: forall A (ls1:list A),
-  ls1 <> nil <-> rev ls1 <> nil.
-Proof.
-  induction ls1; simpl.
-    split; auto.  
-    split; intro J; auto with datatypes v62.      
-Qed.
-
 Section create_dtree__wf_dtree.
 
 Variable dts: PMap.t LDoms.t.
@@ -633,7 +126,7 @@ Variable res: positive -> LDoms.t.
 Hypothesis Hquery: res = fun p:positive => PMap.get p dts.
 Variable rd: list positive.
 Hypothesis Hreach: forall p, PCfg.reachable psuccs pe p -> List.In p rd.
-Variable dt: DTree.
+Variable dt: @DTree positive.
 Hypothesis Hdtree: create_dtree pe rd res = dt.
 Hypothesis wf_entrypoints: in_cfg psuccs pe.
 Definition entrypoints := (pe, LDoms.top) :: nil.
@@ -645,7 +138,7 @@ Hypothesis Hok: pdom_analysis_is_successful psuccs pe.
 Hypothesis Hnopred: (XPTree.make_predecessors psuccs) ??? pe = nil.
 
 Lemma create_dtree__wf_dtree: forall p0 ch0,
-  is_dtree_edge dt p0 ch0 = true <-> 
+  is_dtree_edge positive_eq_dec dt p0 ch0 = true <-> 
     (PCfg.imm_domination psuccs pe p0 ch0 /\ PCfg.reachable psuccs pe ch0).
 Proof.
   intros.
@@ -738,7 +231,7 @@ Fixpoint dtree_dom (dt: DTree) : positives :=
 match dt with
 | DT_node l0 dts0 => union (singleton l0) (dtrees_dom dts0)
 end
-with dtrees_dom (dts: DTrees) : positives :=
+with dtrees_dom (dts: @DTrees positive) : positives :=
 match dts with
 | DT_nil => PositiveSetImpl.empty
 | DT_cons dt0 dts0 => union (dtree_dom dt0) (dtrees_dom dts0)
@@ -746,11 +239,13 @@ end.
 
 Definition in_dtree_dom__in_dtree_insert_dom_prop (dt:DTree) :=
 forall i0 p ch tl,
-  In i0 (dtree_dom dt) -> In i0 (dtree_dom (dtree_insert dt p ch tl)).
+  In i0 (dtree_dom dt) -> 
+  In i0 (dtree_dom (dtree_insert positive_eq_dec dt p ch tl)).
 
 Definition in_dtrees_dom__in_dtrees_insert_dom_prop (dts:DTrees) :=
 forall i0 ch tl,
-  In i0 (dtrees_dom dts) -> In i0 (dtrees_dom (dtrees_insert dts ch tl)).
+  In i0 (dtrees_dom dts) -> 
+  In i0 (dtrees_dom (dtrees_insert positive_eq_dec dts ch tl)).
 
 Lemma in_dtree_dom__in_dtree_insert_dom_mutrec :
   (forall dt, in_dtree_dom__in_dtree_insert_dom_prop dt) *
@@ -761,7 +256,7 @@ Proof.
            in_dtrees_dom__in_dtrees_insert_dom_prop;
     simpl; intros.
   Case "DT_node".
-  destruct (positive_eq_dec p0 p); subst; simpl; auto.
+  destruct (positive_eq_dec p a); subst; simpl; auto.
     apply PositiveSetFacts.union_iff in H0.
     apply PositiveSetFacts.union_iff. 
     destruct H0; auto.
@@ -786,7 +281,8 @@ Proof.
 Qed.
 
 Lemma in_dtree_dom__in_dtree_insert_dom: forall dt i0 p ch tl,
-  In i0 (dtree_dom dt) -> In i0 (dtree_dom (dtree_insert dt p ch tl)).
+  In i0 (dtree_dom dt) -> 
+  In i0 (dtree_dom (dtree_insert positive_eq_dec dt p ch tl)).
 Proof.
   destruct in_dtree_dom__in_dtree_insert_dom_mutrec as [H _].
   unfold in_dtree_dom__in_dtree_insert_dom_prop in H. auto.
