src3.0/Vellvm/Dominators/dom_tree.v
@@ -1,0 +1,1177 @@
+Require Import Coqlib.
+Require Import Metatheory.
+Require Import infrastructure_props.
+Require Import cfg.
+Require Import Relations.Relation_Operators.
+
+Section DTree.
+
+Variable A:Set.
+Hypothesis Hdec: forall x y:A, {x = y} + {x <> y}.
+
+Inductive DTree : Set :=
+| DT_node : A -> DTrees -> DTree
+with DTrees : Set :=
+| DT_nil : DTrees
+| DT_cons : DTree -> DTrees -> DTrees
+.
+
+Fixpoint size_of_dtrees (dts:DTrees) : nat :=
+match dts with
+| DT_nil => O
+| DT_cons _ dts' => S (size_of_dtrees dts')
+end.
+
+Fixpoint list2tree hd tl := 
+match tl with
+| nil => DT_node hd DT_nil
+| hd'::tl' => DT_node hd (DT_cons (list2tree hd' tl') DT_nil)
+end.
+
+Fixpoint dtree_insert dt parent child tl : DTree :=
+match dt with
+| DT_node l0 dts0 =>
+    if Hdec parent l0
+    then DT_node l0 (dtrees_insert dts0 child tl)
+    else dt
+end
+with dtrees_insert (dts: DTrees) child tl : DTrees :=
+match dts with
+| DT_nil => DT_cons (list2tree child tl) DT_nil
+| DT_cons dt0 dts0 =>
+    let '(DT_node l0 _) := dt0 in
+    if Hdec l0 child then 
+      match tl with
+      | child'::tl' => DT_cons (dtree_insert dt0 child child' tl') dts0
+      | _ => dts
+      end
+    else DT_cons dt0 (dtrees_insert dts0 child tl)
+end.
+
+Definition create_dtree_from_chain dt chain : DTree :=
+match chain with
+| p::(ch::chain') => dtree_insert dt p ch chain'
+| _ => dt
+end.
+
+Fixpoint in_children_roots child dts : bool :=
+match dts with
+| DT_nil => false
+| DT_cons (DT_node l0 _) dts' =>
+    if (Hdec l0 child) then true else in_children_roots child dts'
+end.
+
+Fixpoint is_dtree_edge dt parent child : bool :=
+match dt with
+| DT_node l0 dts0 =>
+    if (Hdec parent l0) then
+      if in_children_roots child dts0 then true
+      else is_dtrees_edge dts0 parent child
+    else is_dtrees_edge dts0 parent child
+end
+with is_dtrees_edge (dts: DTrees) parent child : bool :=
+match dts with
+| DT_nil => false
+| DT_cons dt0 dts0 =>
+    is_dtree_edge dt0 parent child || is_dtrees_edge dts0 parent child
+end.
+
+Scheme dtree_rec2 := Induction for DTree Sort Set
+  with dtrees_rec2 := Induction for DTrees Sort Set.
+
+Definition dtree_mutrec P P' :=
+  fun h1 h2 h3 =>
+    (pair (@dtree_rec2 P P' h1 h2 h3) (@dtrees_rec2 P P' h1 h2 h3)).
+
+Fixpoint is_chain_edge (chain:list A) p0 ch0 : Prop :=
+match chain with
+| p::((ch::_) as chain') => (p = p0 /\ ch = ch0) \/ is_chain_edge chain' p0 ch0
+| _ => False
+end.
+
+Lemma dtrees_insert__in_children_roots: forall ch ch0 tl dts
+  (Hin: in_children_roots ch dts = true),
+  in_children_roots ch (dtrees_insert dts ch0 tl) = true.
+Proof.
+  induction dts as [|[]]; simpl; intro; try congruence.
+    destruct_if.
+      destruct_if.
+        destruct tl; simpl.
+          destruct_if.
+          destruct_if. destruct_if.
+        simpl. destruct_if.
+      destruct_if.
+        destruct tl; simpl.
+          destruct_if.
+          destruct_if; try congruence.
+            destruct_if.
+        simpl. 
+        destruct_if.
+          rewrite IHdts; auto.
+Qed.
+
+Lemma list2tree_spec: forall ch0 tl,
+  exists dts, list2tree ch0 tl = DT_node ch0 dts.
+Proof.
+  destruct tl; simpl; eauto.
+Qed.
+
+Lemma inserted_in_children_roots: forall ch ch0 tl dts
+  (Hnotin: in_children_roots ch dts = false)
+  (Hin: in_children_roots ch (dtrees_insert dts ch0 tl) = true),
+  ch = ch0.
+Proof.
+  induction dts as [|[]]; simpl; intros.
+  Case "1".
+    destruct (list2tree_spec ch0 tl) as [dts Heq].
+    rewrite Heq in Hin.
+    destruct_if; try solve [auto | congruence].
+  Case "2".
+    destruct_if.
+    SCase "2.1".
+      destruct_if; try congruence.
+      destruct_if.
+      destruct tl; simpl in *.
+        destruct_if; try congruence.
+        destruct_if; try congruence.
+    SCase "2.2".
+      destruct_if; try solve [congruence | auto].
+Qed.
+
+Lemma inserted_in_children_roots': forall ch0 tl dts,
+  in_children_roots ch0 (dtrees_insert dts ch0 tl) = true.
+Proof.
+  induction dts as [|[]]; simpl; intros.
+  Case "1".
+    destruct (list2tree_spec ch0 tl) as [dts Heq].
+    rewrite Heq.
+    destruct_if; try solve [auto | congruence].
+  Case "2".
+    destruct_if.
+    SCase "2.1".
+      destruct_if; try congruence.
+      destruct tl; simpl in *.
+        destruct_if; try congruence.
+        destruct_if; try congruence.
+    SCase "2.2".
+      simpl. destruct_if; try solve [congruence | auto].
+Qed.
+
+Definition get_dtree_root (dt:DTree) : A :=
+match dt with
+| DT_node l0 _ => l0
+end.
+
+Definition dtree_insert__is_dtree_edge_prop (dt:DTree) :=
+forall p ch tl p0 ch0,
+  is_dtree_edge (dtree_insert dt p ch tl) p0 ch0 = true <->
+  is_dtree_edge dt p0 ch0 = true \/ 
+    (p = get_dtree_root dt /\ is_chain_edge (p::ch::tl) p0 ch0).
+
+Definition dtrees_insert__is_dtrees_edge_prop (dts:DTrees) :=
+forall ch tl p0 ch0,
+  is_dtrees_edge (dtrees_insert dts ch tl) p0 ch0 = true <->
+  is_dtrees_edge dts p0 ch0 = true \/ is_chain_edge (ch::tl) p0 ch0.
+
+Lemma is_dtrees_egde_cons_elim: forall dt1 dts2 p ch
+  (Hin: is_dtrees_edge (DT_cons dt1 dts2) p ch = true),
+  is_dtree_edge dt1 p ch = true \/ is_dtrees_edge dts2 p ch = true.
+Proof.
+  simpl.
+  intros.
+  binvt Hin as J1 J2; auto.
+Qed.
+
+Lemma is_dtrees_egde_cons_intro: forall dt1 dts2 p ch
+  (Hin: is_dtree_edge dt1 p ch = true \/ is_dtrees_edge dts2 p ch = true),
+  is_dtrees_edge (DT_cons dt1 dts2) p ch = true.
+Proof.
+  simpl.
+  intros. auto with datatypes v62.
+Qed.
+
+Lemma DT_nil_has_no_dtree_edges: forall p ch,
+  is_dtrees_edge DT_nil p ch = false.
+Proof. simpl. auto. Qed.
+
+Lemma single_node_has_no_dtree_edges: forall hd p ch,
+  is_dtree_edge (DT_node hd DT_nil) p ch = false.
+Proof. intros. simpl. destruct_if. Qed.
+
+Lemma is_dtree_edge_of_list2tree__is_chain_edge: forall p0 ch0 tl ch
+  (Hin: is_dtree_edge (list2tree ch tl) p0 ch0 = true),
+  is_chain_edge (ch::tl) p0 ch0.
+Proof.
+Local Opaque is_dtrees_edge.
+  induction tl as [|hd tl']; simpl; intros.
+    destruct_if; congruence.
+
+    destruct_if.
+      destruct (list2tree_spec hd tl') as [x Heq].
+      rewrite Heq in H0.
+      destruct (Hdec hd ch0); subst; auto.
+        apply is_dtrees_egde_cons_elim in H0.
+        destruct H0 as [H0 | H0].
+          right. apply IHtl'. rewrite Heq. auto.
+
+          rewrite DT_nil_has_no_dtree_edges in H0. congruence.
+       apply is_dtrees_egde_cons_elim in H0.
+       destruct H0 as [H0 | H0].
+         right. apply IHtl'. auto.
+         rewrite DT_nil_has_no_dtree_edges in H0. congruence.
+Qed.
+
+Lemma is_chain_edge__is_dtree_edge_of_list2tree: forall p0 ch0 tl ch
+  (Hin: is_chain_edge (ch::tl) p0 ch0),
+  is_dtree_edge (list2tree ch tl) p0 ch0 = true.
+Proof.
+  induction tl as [|hd tl']; simpl; intros.
+    tauto.
+
+    destruct (list2tree_spec hd tl') as [x Heq].
+    rewrite Heq.
+    destruct Hin as [[EQ1 EQ2] | Hin]; subst.
+      destruct_if.
+      destruct (Hdec ch0 ch0); try congruence.
+
+      destruct (Hdec p0 ch); subst.
+        destruct (Hdec hd ch0); subst; auto.
+          apply is_dtrees_egde_cons_intro.
+          left. rewrite <- Heq. apply IHtl'; auto.          
+
+        apply is_dtrees_egde_cons_intro.
+        left. rewrite <- Heq. apply IHtl'; auto.          
+Transparent is_dtrees_edge.
+Qed.
+
+Lemma dtree_insert__is_dtree_edge_mutrec :
+  (forall dt, dtree_insert__is_dtree_edge_prop dt) *
+  (forall dts, dtrees_insert__is_dtrees_edge_prop dts).
+Proof.
+  apply dtree_mutrec;
+    unfold dtree_insert__is_dtree_edge_prop, dtrees_insert__is_dtrees_edge_prop;
+    intros; simpl.
+  Case "DT_node".
+    destruct_if.
+    SCase "p0 = root".
+      destruct_if.
+      SSCase "p1 = root".
+        remember (in_children_roots ch0 d) as R.
+        destruct R; simpl.
+        SSSCase "ch0 in d".
+          destruct_if; try congruence.
+          split; intro J; auto.
+            rewrite dtrees_insert__in_children_roots; auto.
+
+        SSSCase "ch0 notin d".
+          destruct_if; try congruence.
+          remember (in_children_roots ch0 (dtrees_insert d ch tl)) as R.
+          destruct R; simpl.
+          SSSSCase "ch0 in inserted".
+            split; intro; auto.
+              right.
+              split; auto.
+                left.
+                split; auto.
+                  symmetry in HeqR3.
+                  eapply inserted_in_children_roots in HeqR3; eauto.
+          SSSSCase "ch0 notin inserted".
+            split; intro J.
+            SSSSSCase "1".
+              apply H in J.
+              destruct J as [J | J]; auto.
+            SSSSSCase "2".
+              apply H. 
+              destruct J as [J | [J1 [[EQ1 EQ2] |J2]]]; subst; auto.
+                rewrite inserted_in_children_roots' in HeqR3. congruence.
+      SSCase "p1 <> root".
+        simpl.
+        destruct_if; try congruence.
+        split; intro J.
+          SSSCase "1".
+            apply H in J.
+            destruct J as [J | J]; auto.
+          SSSCase "2".
+            apply H. 
+            destruct J as [J | [J1 [[EQ1 EQ2] |J2]]]; subst; auto.
+    SCase "p0 <> root".
+      simpl.
+      destruct_if.
+      SSCase "p1 = root".
+        split; intro J; auto.
+          SSSCase "1".
+          remember (in_children_roots ch0 d) as R.
+          destruct R; simpl; auto.
+            destruct J as [J | [J1 [[EQ1 EQ2] |J2]]]; subst; auto.
+      SSCase "p1 <> root".
+        split; intro J; auto.
+          destruct J as [J | [J1 [[EQ1 EQ2] |J2]]]; subst; auto.
+
+  Case "DT_nil".
+    split; intros J.
+      bdestruct J as J1 J2; try congruence.
+        right.
+        apply is_dtree_edge_of_list2tree__is_chain_edge; auto.
+     destruct J as [J | J]; try congruence.
+
+      rewrite is_chain_edge__is_dtree_edge_of_list2tree; auto.
+
+  Case "DT_cons".
+    destruct d as [l0 ?].
+    destruct_if.
+    SCase "l0 = ch".
+      destruct tl; try tauto.
+      SSCase "tl<>nil".
+        split; intro J.
+        SSSCase "1".
+          apply is_dtrees_egde_cons_elim in J.
+          destruct J as [J | J].
+          SSSSCase "1.1".
+            apply H in J. 
+            destruct J as [J1 |[J2 J3]]; auto.
+              rewrite J1. auto.
+          SSSSCase "1.2".
+            left. rewrite J. auto with datatypes v62.
+        SSSCase "2".
+          apply is_dtrees_egde_cons_intro.
+          destruct J as [J | [[J1 J2] | J]]; subst.
+          SSSSCase "2.1".
+            binvt J as J1 J2; auto.
+              left. apply H; auto.
+          SSSSCase "2.2".
+            left. apply H; simpl; auto.
+          SSSSCase "2.3".
+            left. apply H; simpl; auto.
+    SCase "l0 <> ch".
+        split; intro J.
+        SSSCase "1".
+          apply is_dtrees_egde_cons_elim in J.
+          destruct J as [J | J].
+          SSSSCase "1.1".
+            left.
+            apply is_dtrees_egde_cons_intro; auto.
+          SSSSCase "1.2".
+            apply H0 in J.
+            destruct J as [J | J].
+              left. apply is_dtrees_egde_cons_intro; auto.
+              right. auto.
+        SSSCase "2".
+          apply is_dtrees_egde_cons_intro.
+          destruct J as [J | J].    
+          SSSSCase "2.1".
+            binvt J as J1 J2; auto.
+              right. apply H0; auto.
+          SSSSCase "2.2".
+            right. apply H0; auto.
+Qed.
+
+Lemma dtree_insert__is_dtree_edge : forall p ch tl p0 ch0 dt,
+  is_dtree_edge (dtree_insert dt p ch tl) p0 ch0 = true <->
+  is_dtree_edge dt p0 ch0 = true \/ 
+  p = get_dtree_root dt /\ is_chain_edge (p::ch::tl) p0 ch0.
+Proof.
+  destruct (dtree_insert__is_dtree_edge_mutrec).
+  unfold dtree_insert__is_dtree_edge_prop in *.
+  eauto.
+Qed.
+
+Definition chain_connects_dtree dt (chain:list A) : Prop :=
+match chain with
+| entry :: _ :: _ => entry = get_dtree_root dt
+| _ => False
+end.
+
+Lemma dtree_insert__get_dtree_root: forall dt p ch tl,
+  get_dtree_root dt = get_dtree_root (dtree_insert dt p ch tl).
+Proof.
+  destruct dt; simpl.
+  intros.
+  destruct_if; auto.
+Qed.
+
+Lemma create_dtree_from_chain__is_dtree_edge__is_chain_edge:
+  forall p0 ch0 chain dt,
+  (is_dtree_edge (create_dtree_from_chain dt chain) p0 ch0 = true ->
+   is_dtree_edge dt p0 ch0 = true \/ is_chain_edge chain p0 ch0) /\
+  (is_dtree_edge dt p0 ch0 = true \/
+   (chain_connects_dtree dt chain /\ is_chain_edge chain p0 ch0) ->
+   is_dtree_edge (create_dtree_from_chain dt chain) p0 ch0 = true).
+Proof.
+  intros.
+Local Opaque is_chain_edge.
+  destruct chain as [|p chain]; simpl; try tauto.
+  destruct chain as [|ch chain]; simpl; try tauto.
+  split; intros.
+    apply dtree_insert__is_dtree_edge in H. tauto.
+    apply dtree_insert__is_dtree_edge in H; auto.
+Transparent is_chain_edge.
+Qed.
+
+Lemma create_dtree_from_chain__chain_connects_dtree: forall chain0 chain dt
+  (H: chain_connects_dtree dt chain0),
+  chain_connects_dtree (create_dtree_from_chain dt chain) chain0.
+Proof.
+  intros.
+  destruct chain0 as [|p0 chain0]; auto.
+  destruct chain0 as [|ch0 chain0]; auto.
+  simpl in *.
+  destruct chain as [|p chain]; auto.
+  destruct chain as [|ch chain]; auto.
+  subst. apply dtree_insert__get_dtree_root.
+Qed.
+
+Lemma fold_left_create_dtree_from_chain__is_dtree_edge__is_chain_edge:
+  forall p0 ch0 chains dt,
+  (is_dtree_edge
+    (fold_left
+      (fun (acc : DTree) (elt : A * list A) =>
+       let '(_, chain) := elt in create_dtree_from_chain acc chain)
+     chains dt) p0 ch0 = true ->
+  (is_dtree_edge dt p0 ch0 = true \/
+   exists l0, exists chain0,
+     List.In (l0, chain0) chains /\ is_chain_edge chain0 p0 ch0)) /\
+  ((is_dtree_edge dt p0 ch0 = true \/
+   exists l0, exists chain0,
+     List.In (l0, chain0) chains /\ chain_connects_dtree dt chain0 /\
+     is_chain_edge chain0 p0 ch0) ->
+   is_dtree_edge
+    (fold_left
+      (fun (acc : DTree) (elt : A * list A) =>
+       let '(_, chain) := elt in create_dtree_from_chain acc chain)
+     chains dt) p0 ch0 = true).
+Proof.
+  induction chains as [|[p l1] chains]; simpl; intros.
+    split; intro J; auto.
+      destruct J as [H | [l0 [chn0 [J1 J2]]]]; auto.
+
+    destruct (IHchains (create_dtree_from_chain dt l1)) as [J1 J2].
+    clear IHchains.
+    split; intros J.
+      apply J1 in J.
+      destruct J as [J | [l2 [chain2 [J3 J4]]]].
+        apply create_dtree_from_chain__is_dtree_edge__is_chain_edge in J.
+        destruct J as [J | J]; auto.
+          right. eauto. 
+        right. exists l2. exists chain2. auto.
+
+      apply J2.
+      destruct J as [J | [l2 [chain2 [J3 [J4 J5]]]]].
+        left.
+        apply create_dtree_from_chain__is_dtree_edge__is_chain_edge; auto.
+
+        destruct J3 as [J3 | J3].
+          inv J3. left.
+          apply create_dtree_from_chain__is_dtree_edge__is_chain_edge; auto.
+
+          right. exists l2. exists chain2. split; auto. split; auto.
+            apply create_dtree_from_chain__chain_connects_dtree; auto.
+Qed.
+
+Lemma is_chain_edge_tail: forall p0 ch0 ls2 ls1 
+  (Hintl: is_chain_edge ls2 p0 ch0),
+  is_chain_edge (ls1 ++ ls2) p0 ch0.
+Proof.
+  induction ls1; simpl; intros; auto.
+    case_eq (ls1 ++ ls2).
+      intro J.
+      apply app_eq_nil in J. 
+      destruct J; subst; simpl in Hintl; auto.
+
+      intros p l EQ.
+      rewrite <- EQ. auto.
+Qed.
+
+Lemma chain_edge_sorted: forall R p0 ch0 ls1 (Hedge: is_chain_edge ls1 p0 ch0)
+  (Hsort : Sorted R ls1), R p0 ch0.
+Proof.
+  induction 2; simpl in *.
+    tauto.
+
+    destruct l; try tauto.   
+    destruct Hedge as [[EQ1 EQ2] | Hedge]; subst; auto.
+      inv H. auto.
+Qed.
+
+Lemma is_chain_edge__inv: forall p0 ch0 l0 dts0
+  (Hedge: is_chain_edge (dts0 ++ [l0]) p0 ch0),
+  In p0 (dts0 ++ [l0]) /\ In ch0 (dts0 ++ [l0]) /\ dts0 <> nil.
+Proof.
+  induction dts0; simpl; intros.
+    tauto.
+
+    case_eq (dts0 ++ [l0]).
+      intro Heq.
+      destruct dts0; inv Heq.
+
+      intros p1 l1 Heq.
+      rewrite Heq in Hedge.
+      destruct Hedge as [[EQ1 EQ2] | Hedge]; subst.
+        simpl. 
+        split; auto.
+        split; auto.
+          congruence.
+
+        rewrite <- Heq in *.
+        apply IHdts0 in Hedge.
+        destruct Hedge as [J1 [J2 J3]].
+        split; auto.
+        split; auto.
+          congruence.     
+Qed.
+
+Import AtomSet.
+Import ListSet.
+
+Fixpoint dtree_dom (dt: DTree) : set A :=
+match dt with
+| DT_node l0 dts0 => set_add Hdec l0 (dtrees_dom dts0)
+end
+with dtrees_dom (dts: DTrees) : set A :=
+match dts with
+| DT_nil => @empty_set A
+| DT_cons dt0 dts0 => set_union Hdec (dtree_dom dt0) (dtrees_dom dts0)
+end.
+
+Fixpoint disjoint_dtrees (dts: DTrees): Prop :=
+match dts with
+| DT_nil => True
+| DT_cons dt dts' => set_disjoint Hdec (dtree_dom dt) (dtrees_dom dts') /\
+                     disjoint_dtrees dts'
+end.
+
+Inductive uniq_dtree : DTree -> Prop :=
+| U_DT_node : forall p dts
+            (Hnotin: ~ In p (dtrees_dom dts))
+            (Hdisj: disjoint_dtrees dts)
+            (Hwfdts: uniq_dtrees dts),
+            uniq_dtree (DT_node p dts)
+with uniq_dtrees : DTrees -> Prop :=
+| U_DT_nil : uniq_dtrees DT_nil
+| U_DT_cons : forall dt dts (Hwfdt: uniq_dtree dt) (Hwfdts: uniq_dtrees dts),
+                 uniq_dtrees (DT_cons dt dts)
+.
+
+Fixpoint get_dtrees_roots dts : set A :=
+match dts with
+| DT_nil => @empty_set A
+| DT_cons dt' dts' => set_add Hdec (get_dtree_root dt') (get_dtrees_roots dts')
+end.
+
+Fixpoint disjoint_dtrees_roots dts : Prop :=
+match dts with
+| DT_nil => True
+| DT_cons dt' dts' => ~ In (get_dtree_root dt') (get_dtrees_roots dts') /\
+                      disjoint_dtrees_roots dts'
+end.
+
+Inductive disjoint_children_dtree : DTree -> Prop :=
+| Dj_DT_node : forall p dts             
+               (Hwfdts: disjoint_children_dtrees dts),
+               disjoint_children_dtree (DT_node p dts)
+with disjoint_children_dtrees : DTrees -> Prop :=
+| Dj_DT_nil : disjoint_children_dtrees DT_nil
+| Dj_DT_cons : forall dt dts (Hwfdt: disjoint_children_dtree dt) 
+               (Hwfdts: disjoint_children_dtrees dts)
+               (Hdisj: disjoint_dtrees_roots (DT_cons dt dts)),
+               disjoint_children_dtrees (DT_cons dt dts)
+.
+
+Definition dtree_is_sound (dt:DTree) (idom: A -> A -> Prop): Prop :=
+  forall p ch (Hedge: is_dtree_edge dt p ch = true),
+    exists chain, is_chain_edge chain p ch /\ 
+    Sorted idom chain /\ NoDup chain.
+
+Definition dtrees_is_sound (dts:DTrees) (idom: A -> A -> Prop) : Prop :=
+  forall p ch (Hedge: is_dtrees_edge dts p ch = true),
+    exists chain, is_chain_edge chain p ch /\ 
+    Sorted idom chain /\ NoDup chain.
+
+Fixpoint in_children (dt: DTree) dts : Prop :=
+match dts with
+| DT_nil => False
+| DT_cons dt' dts' => dt = dt' \/ in_children dt dts'
+end.
+
+Require Import Dipaths.
+
+Definition dvertexes (dt: DTree) : V_set := 
+fun (v:Vertex) => let '(index n) := v in In n (dtree_dom dt).
+
+Definition darcs (dt: DTree) : A_set := 
+fun (arc:Arc) =>
+  let '(A_ends (index n2) (index n1)) := arc in
+  is_dtree_edge dt n1 n2 = true.
+
+Definition dtree_walk (dt: DTree) (n:A) : Prop :=
+  exists vl, exists al, 
+    D_walk (dvertexes dt) (darcs dt) (index n) (index (get_dtree_root dt)) vl al.
+
+Lemma DT_cons_hd_extends_darcs: forall l1 d dts (x : Arc)
+  (Hinx: darcs (DT_node l1 dts) x), darcs (DT_node l1 (DT_cons d dts)) x.
+Proof.
+  intros.
+  destruct x as [[a] [b]]. simpl in *.
+  destruct_if.
+    rewrite H0.
+    destruct d.
+    destruct_if.
+      destruct_if.
+      destruct_if.
+  
+      rewrite H1.
+      destruct_if; auto with datatypes v62.
+  
+    rewrite H0. auto with datatypes v62.
+Qed.
+
+Lemma DT_cons_hd_extends_dvertexes: forall l1 d dts (x : Vertex)
+  (Hinx: dvertexes (DT_node l1 dts) x), dvertexes (DT_node l1 (DT_cons d dts)) x.
+Proof.
+  intros.
+  destruct x as [x]. simpl in *.
+  apply set_add_elim in Hinx.
+  destruct Hinx; subst.
+    apply set_add_intro2; auto.
+  
+    apply set_add_intro1.
+    apply set_union_intro; auto.
+Qed.
+
+Lemma DT_cons_tl_extends_dvertexes: forall l1 d dts (x : Vertex)
+  (Hinx: dvertexes d x), dvertexes (DT_node l1 (DT_cons d dts)) x.
+Proof.
+  intros.
+  destruct x as [x].
+  simpl in *.
+  apply set_add_intro1.
+  apply set_union_intro; auto.
+Qed.
+
+Lemma DT_cons_tl_extends_darcs: forall l1 d dts (x : Arc)
+  (Hinx: darcs d x), darcs (DT_node l1 (DT_cons d dts)) x.
+Proof.
+  intros.
+  destruct x as [[a] [b]]. simpl in *.
+  rewrite Hinx. 
+  destruct_if.
+  destruct d.
+  destruct_if.
+Qed.
+
+Lemma get_dtree_root_in_dtree_dom: forall dt,
+  In (get_dtree_root dt) (dtree_dom dt).
+Proof.
+  destruct dt; simpl.
+  apply set_add_intro2; auto.
+Qed.
+
+Lemma dtree_child_walk__dtree_walk: forall l1 l2 dt dts 
+  (Hinch : in_children dt dts)
+  (Hwk : dtree_walk dt l2),
+  dtree_walk (DT_node l1 dts) l2.
+Proof.
+  induction dts; simpl; intros.
+    tauto.
+
+    destruct Hinch as [Hinch | Hinch]; subst.
+      destruct Hwk as [vl [al Hwk]].
+      exists (vl++[index l1]).
+      exists (al++[A_ends (index (get_dtree_root d)) (index l1)]).
+      apply DWalk_append with (y:=index (get_dtree_root d)); auto.
+        eapply D_walk_sub in Hwk; eauto.
+         apply DT_cons_tl_extends_dvertexes.
+         apply DT_cons_tl_extends_darcs.
+
+        simpl.
+        apply DW_step; simpl.
+          constructor; simpl.
+            apply set_add_intro2; auto.
+          apply set_add_intro1; auto.
+            apply set_union_intro. left.
+            apply get_dtree_root_in_dtree_dom.
+
+          destruct_if.
+          destruct d. simpl.
+          destruct_if.
+          destruct_if. congruence.
+ 
+       apply IHdts in Hinch; auto.
+       destruct Hinch as [vl [al Hinch]].
+       exists vl. exists al.
+       simpl in *.
+       eapply D_walk_sub in Hinch; eauto.
+         apply DT_cons_hd_extends_dvertexes.
+         apply DT_cons_hd_extends_darcs.
+Qed.
+
+Definition in_dtree_dom__is_dtree_walk_prop (dt:DTree) :=
+  forall l0 (Hin: In l0 (dtree_dom dt)), dtree_walk dt l0.
+
+Definition in_dtrees_dom__is_dtrees_walk_prop (dts:DTrees) :=
+  forall l0 (Hin: In l0 (dtrees_dom dts)), 
+  exists dt, in_children dt dts /\ dtree_walk dt l0.
+
+Lemma in_dtree_dom__is_dtree_walk_mutrec :
+  (forall dt, in_dtree_dom__is_dtree_walk_prop dt) *
+  (forall dts, in_dtrees_dom__is_dtrees_walk_prop dts).
+Proof.
+  apply dtree_mutrec;
+    unfold in_dtree_dom__is_dtree_walk_prop, in_dtrees_dom__is_dtrees_walk_prop;
+    simpl; intros; try tauto.
+  Case "DT_node".
+    apply set_add_elim in Hin.
+    destruct Hin as [Hin | Hin]; subst.
+      exists V_nil. exists A_nil. simpl.
+      constructor; auto.
+        simpl. apply set_add_intro2; auto.
+
+      apply H in Hin.
+      destruct Hin as [dt [J1 J2]].
+      eapply dtree_child_walk__dtree_walk; eauto.
+  Case "DT_cons".
+    apply set_union_elim in Hin.
+    destruct Hin as [Hin | Hin]; eauto.
+      apply H0 in Hin. 
+      destruct Hin as [dt [J1 J2]].
+      eauto.
+Qed.
+
+Lemma in_dtree_dom__is_dtree_walk: forall dt l0 (Hin: In l0 (dtree_dom dt)),
+  dtree_walk dt l0.
+Proof.
+  intros.
+  destruct in_dtree_dom__is_dtree_walk_mutrec as [J1 J2].
+  apply J1; auto.
+Qed.
+
+Lemma in_dtrees_dom__is_dtree_walk: forall dts l0 (Hin: In l0 (dtrees_dom dts)),
+  exists dt, in_children dt dts /\ dtree_walk dt l0.
+Proof.
+  intros.
+  destruct in_dtree_dom__is_dtree_walk_mutrec as [J1 J2].
+  apply J2; auto.
+Qed.
+
+Lemma in_children__in_children_roots: forall dt dts (Hin: in_children dt dts),
+  in_children_roots (get_dtree_root dt) dts = true.
+Proof.
+  induction dts as [|[] dts]; simpl; intros; auto.
+    destruct_if.
+    destruct Hin as [Hin | HIn]; subst; simpl in *; auto.
+Qed.
+
+Fixpoint forall_parent_children (R:A -> A -> Prop) (p:A) (dts:DTrees) 
+  : Prop :=
+match dts with
+| DT_nil => True
+| DT_cons dt dts' => R p (get_dtree_root dt) /\ 
+                     forall_parent_children R p dts'
+end.
+
+Lemma forall_parent_children__in_children: forall R p dt dts
+  (Hforall: forall_parent_children R p dts)
+  (Hin: in_children dt dts),
+  R p (get_dtree_root dt).
+Proof.
+  induction dts; simpl; intros.
+    tauto.
+    destruct Hin as [Hin | Hin]; subst; tauto.
+Qed.
+
+Lemma in_children__forall_parent_children: forall (R:A->A->Prop) p dts
+  (Hp: forall dt (Hin: in_children dt dts), R p (get_dtree_root dt)),
+  forall_parent_children R p dts.
+Proof.
+  induction dts; simpl; intros; auto.
+Qed.
+
+Lemma in_children__is_dtree_edge: forall l0 dt dts (Hin : in_children dt dts),
+  is_dtree_edge (DT_node l0 dts) l0 (get_dtree_root dt) = true.
+Proof.
+  induction dts as [|[] dts]; simpl; intros.
+    tauto.
+
+    destruct Hin as [Hin | Hin]; subst; simpl in *.
+      repeat destruct_if.
+
+      repeat destruct_if;
+        rewrite IHdts; auto with datatypes v62.
+Qed.
+
+Lemma dtree_edge_sorted: forall R dt p ch
+  (Hp : dtree_is_sound dt R) (Hedge: is_dtree_edge dt p ch = true),
+  R p ch.
+Proof.
+  intros.
+  apply Hp in Hedge.
+  destruct Hedge as [chain [J1 [J2 J3]]].
+  eapply chain_edge_sorted; eauto.
+Qed.
+
+Lemma DT_node_is_sound_inv: forall R l0 dts
+  (Hp : dtree_is_sound (DT_node l0 dts) R),
+  dtrees_is_sound dts R /\ forall_parent_children R l0 dts.
+Proof.
+  intros.
+  unfold dtree_is_sound, dtrees_is_sound in *.
+  split.
+    intros. apply Hp. simpl.
+    rewrite Hedge.
+    destruct (Hdec p l0); subst; auto.
+    destruct (in_children_roots ch dts); auto.
+
+    apply in_children__forall_parent_children.
+    intros dt Hin.
+    apply in_children__is_dtree_edge with (l0:=l0) in Hin.
+    eapply dtree_edge_sorted; eauto.
+Qed.
+
+Lemma DT_cons_is_sound_inv: forall idom dt dts
+  (Hp : dtrees_is_sound (DT_cons dt dts) idom),
+  dtree_is_sound dt idom /\ dtrees_is_sound dts idom.
+Proof.
+  unfold dtree_is_sound, dtrees_is_sound in *.
+  intros.
+  split; intros.
+    apply Hp. apply is_dtrees_egde_cons_intro; auto.
+    apply Hp. apply is_dtrees_egde_cons_intro; auto.
+Qed.
+
+Lemma dtrees_is_sound__dtree_is_sound: forall dt idom dts
+  (H: dtrees_is_sound dts idom) (Hin: in_children dt dts),
+  dtree_is_sound dt idom.
+Proof.
+  unfold dtree_is_sound, dtrees_is_sound in *.
+  induction dts; simpl; intros.
+    tauto.
+
+    destruct Hin as [Hin | Hin]; subst.
+      apply H. rewrite Hedge. auto.
+ 
+      apply IHdts; auto.
+        intros p0 ch0 Hedge0.
+        apply H. rewrite Hedge0. auto with datatypes v62.
+Qed.
+
+Lemma notin_get_dtrees_roots__neq: forall a dt dts
+  (Hnotin: ~ In a (get_dtrees_roots dts))
+  (Hin: in_children dt dts),
+  a <> get_dtree_root dt.
+Proof.
+  induction dts; simpl; intros.
+    tauto.
+
+    destruct Hin as [Hin | Hin]; subst.
+      intro EQ. subst.
+      apply Hnotin. apply set_add_intro2; auto.
+
+      intro EQ. subst. 
+      apply IHdts; auto.
+        intro J. apply Hnotin. apply set_add_intro1; auto.
+Qed.
+
+Lemma dtree_walk__clos_refl_trans_idom: forall idom dt l1 (Hwk: dtree_walk dt l1)
+  (Hsound: dtree_is_sound dt idom),
+  (clos_refl_trans A idom) (get_dtree_root dt) l1.
+Proof.
+  intros.
+  destruct Hwk as [vl [al Hwk]].
+  remember (index l1) as v1.
+  remember (index (get_dtree_root dt)) as ve.
+  generalize dependent l1.
+  generalize dependent (get_dtree_root dt).
+  induction Hwk; simpl; intros; subst.
+    inv Heqv1.
+    apply rt_refl.
+
+    destruct y as [y].
+    apply rt_trans with (y:=y); eauto.
+      apply rt_step.
+      eapply dtree_edge_sorted in Hsound; eauto.
+Qed.
+
+Lemma dtree_walk__clos_trans_idom: forall idom dt a l1 dts 
+  (Hwk: dtree_walk dt l1)
+  (Hsound: dtree_is_sound (DT_node a dts) idom)
+  (Hinch : in_children dt dts),
+  (clos_trans A idom) a l1.
+Proof.
+  intros.
+  apply DT_node_is_sound_inv in Hsound. destruct Hsound.
+  apply dtree_walk__clos_refl_trans_idom with (idom:=idom )in Hwk; 
+    eauto using dtrees_is_sound__dtree_is_sound.
+  eapply step_clos_refl_trans__clos_trans; eauto.
+    eapply forall_parent_children__in_children; eauto.
+Qed.
+
+End DTree.
+
+Implicit Arguments dtree_insert [A].
+Implicit Arguments dtrees_insert [A].
+Implicit Arguments DTree [A].
+Implicit Arguments DTrees [A].
+Implicit Arguments DT_node [A].
+Implicit Arguments DT_nil [A].
+Implicit Arguments DT_cons [A].
+Implicit Arguments create_dtree_from_chain [A].
+Implicit Arguments is_dtree_edge [A].
+Implicit Arguments is_dtrees_edge [A].
+Implicit Arguments is_chain_edge [A].
+Implicit Arguments chain_connects_dtree [A]. 
+Implicit Arguments 
+  fold_left_create_dtree_from_chain__is_dtree_edge__is_chain_edge [A].
+Implicit Arguments get_dtree_root [A].
+Implicit Arguments in_children_roots [A].
+Implicit Arguments dtree_dom [A].
+Implicit Arguments dtrees_dom [A].
+Implicit Arguments in_children [A].
+Implicit Arguments dtree_is_sound [A].
+Implicit Arguments dtrees_is_sound [A].
+Implicit Arguments disjoint_children_dtree [A].
+Implicit Arguments disjoint_children_dtrees [A].
+Implicit Arguments uniq_dtree [A].
+Implicit Arguments uniq_dtrees [A].
+Implicit Arguments forall_parent_children [A].
+Implicit Arguments disjoint_dtrees [A].
+Implicit Arguments disjoint_dtrees_roots [A].
+Implicit Arguments dtree_walk [A].
+
+Require Import Maps.
+
+Module DTreeProps (T:TREE).
+
+Module TCfg := Cfg(T).
+
+Module XTree := More_Tree_Properties(T).
+
+Section create_dtree__wf_dtree.
+
+Variable succs: T.t (list T.elt).
+Variable entry: T.elt.
+Hypothesis Hdec: forall x y:T.elt, {x = y} + {x <> y}.
+
+Inductive reachable_dtree : @DTree T.elt -> Prop :=
+| Rd_DT_node : forall p dts
+            (Hrd: TCfg.reachable succs entry p) 
+            (Hwfdts: reachable_dtrees dts),
+            reachable_dtree (DT_node p dts)
+with reachable_dtrees : @DTrees T.elt -> Prop :=
+| Rd_DT_nil : reachable_dtrees DT_nil
+| Rd_DT_cons : forall dt dts (Hwfdt: reachable_dtree dt) 
+                 (Hwfdts: reachable_dtrees dts),
+                 reachable_dtrees (DT_cons dt dts)
+.
+
+Lemma reachable_dtree__reachable_root: forall d 
+  (Hreach: reachable_dtree d),
+  TCfg.reachable succs entry (get_dtree_root d).
+Proof.
+  intros. inv Hreach. simpl. auto.
+Qed.
+
+Lemma reachable_dtrees__reachable_root: forall dt dts
+  (Hwfdts : reachable_dtrees dts) (Hinchs : in_children dt dts),
+  TCfg.reachable succs entry (get_dtree_root dt).
+Proof.
+  induction 1; simpl; intros.
+    tauto.
+
+    destruct Hinchs as [EQ | Hinchs]; subst; auto.
+      apply reachable_dtree__reachable_root; auto.
+Qed.
+
+Import AtomSet.
+Import ListSet.
+
+Definition in_dom_tree_is_reachable_prop (dt:DTree) :=
+  forall (Hrd: reachable_dtree dt) x (Hp: In x (dtree_dom Hdec dt)), 
+    TCfg.reachable succs entry x.
+
+Definition in_dom_trees_is_reachable_prop (dts:DTrees) :=
+  forall (Hrd: reachable_dtrees dts) x (Hp: In x (dtrees_dom Hdec dts)), 
+    TCfg.reachable succs entry x.
+
+Lemma in_dom_tree_is_reachable_mutrec :
+  (forall dt, in_dom_tree_is_reachable_prop dt) *
+  (forall dts, in_dom_trees_is_reachable_prop dts).
+Proof.
+  apply dtree_mutrec;
+    unfold in_dom_tree_is_reachable_prop, in_dom_trees_is_reachable_prop;
+    simpl; intros; inv Hrd.
+  Case "NODE".
+    unfold dtree_dom in Hp.
+    apply set_add_elim in Hp.
+    destruct Hp as [Hp | Hp]; subst; auto.
+  Case "NIL".
+    tauto.
+  Case "CONS".
+    unfold dtrees_dom in Hp.
+    apply set_union_elim in Hp.
+    destruct Hp as [Hp | Hp]; auto.
+Qed.
+
+Lemma inter_reachable_dtree_is_reachable: forall dt dts
+  (Hwfdt : reachable_dtree dt) (Hwfdts : reachable_dtrees dts) (x : T.elt) 
+  (Hinx : In x (set_inter Hdec (dtree_dom Hdec dt) (dtrees_dom Hdec dts))),
+  TCfg.reachable succs entry x.
+Proof.
+  intros. 
+  destruct in_dom_tree_is_reachable_mutrec as [J1 J2].
+  unfold in_dom_tree_is_reachable_prop, in_dom_trees_is_reachable_prop in *.
+  apply set_inter_elim in Hinx.
+  destruct Hinx; eauto.
+Qed.
+
+Definition idom := TCfg.imm_domination succs entry.
+Definition sdom := TCfg.strict_domination succs entry.
+
+Inductive wf_dtree : @DTree T.elt -> Prop :=
+| Wf_DT_node : forall p dts
+               (Hrd: TCfg.reachable succs entry p) 
+               (Hnotin: ~ In p (dtrees_dom Hdec dts))
+               (Hdisj: disjoint_dtrees Hdec dts)
+               (Hidom: forall_parent_children idom p dts)
+               (Hwfdts: wf_dtrees dts),
+               wf_dtree (DT_node p dts)
+with wf_dtrees : @DTrees T.elt -> Prop :=
+| Wf_DT_nil : wf_dtrees DT_nil
+| Wf_DT_cons : forall dt dts 
+               (Hwfdt: wf_dtree dt) 
+               (Hwfdts: wf_dtrees dts),
+               wf_dtrees (DT_cons dt dts)
+.
+
+Hypothesis entry_has_no_preds : forall a0
+  (Hin: In entry (XTree.successors_list succs a0)),
+  False.
+
+Lemma dtree_walk__sdom: forall dt a l1 dts 
+  (Hwk: dtree_walk Hdec dt l1)
+  (Hsound: dtree_is_sound Hdec (DT_node a dts) idom)
+  (Hinch : in_children dt dts),
+  sdom a l1.
+Proof.
+  intros.
+  apply TCfg.clos_trans_idom__sdom; auto.
+  eapply dtree_walk__clos_trans_idom with (idom:=idom) in Hwk; eauto.
+Qed.
+
+Definition create_dtree__wf_dtree_prop (dt:DTree) :=
+  forall (Hp: dtree_is_sound Hdec dt idom) (Hdj: disjoint_children_dtree Hdec dt)
+    (Hrd: reachable_dtree dt), 
+    wf_dtree dt.
+
+Definition create_dtree__wf_dtrees_prop (dts:DTrees) :=
+  forall (Hp: dtrees_is_sound Hdec dts idom) 
+    (Hdj: disjoint_children_dtrees Hdec dts)
+    (Hrd: reachable_dtrees dts)
+    (Hidom: exists p, forall_parent_children idom p dts),
+    wf_dtrees dts /\ disjoint_dtrees Hdec dts.
+
+Lemma create_dtree__wf_dtree_mutrec :
+  (forall dt, create_dtree__wf_dtree_prop dt) *
+  (forall dts, create_dtree__wf_dtrees_prop dts).
+Proof.
+  apply dtree_mutrec;
+    unfold create_dtree__wf_dtree_prop, create_dtree__wf_dtrees_prop;
+    simpl; intros.
+  Case "DT_node".
+    assert (dtrees_is_sound Hdec d idom /\
+            forall_parent_children idom a d) as Hp'.
+      apply DT_node_is_sound_inv in Hp; auto.
+    inv Hdj. inv Hrd.
+    assert (exists p : T.elt, forall_parent_children idom p d) as Hsdom.
+      exists a. tauto.
+    constructor; try solve [auto | eapply H; eauto | tauto].
+    SCase "1".
+      destruct (In_dec Hdec a (dtrees_dom Hdec d)) as [Hin | Hnotin]; 
+        auto.  
+      elimtype False.
+      apply in_dtrees_dom__is_dtree_walk in Hin.
+      destruct Hin as [dt [Hinch Hwk]].
+      destruct Hp' as [J1 J2].
+      assert (sdom a a) as Hfalse.
+        eapply dtree_walk__sdom with (a:=a) in Hwk; eauto.
+      apply TCfg.sdom_isnt_refl in Hfalse; auto.
+
+  Case "DT_nil".
+    split; auto.
+      constructor.
+  Case "DT_cons".
+    inv Hdj. inv Hrd.
+    assert (Hp':=Hp).
+    apply DT_cons_is_sound_inv in Hp'.   
+    destruct Hp' as [Hp1 Hps2]. 
+    assert (Hsd1:=Hp1). assert (Hsds2:=Hps2).
+    destruct Hidom as [p [Hidom1 Hidoms2]].
+    apply_clear H0 in Hps2; eauto. destruct Hps2 as [Huniqs Hdisjs].
+    apply_clear H in Hp1. 
+    split.
+    SCase "uniq".
+      constructor; eauto.
+    SCase "disjoint".
+      split; auto.
+        split; intros x Hinx; tinv Hinx.
+        elimtype False.
+        assert (J:=Hinx).
+        apply set_inter_elim in J.
+        destruct J as [Hin1 Hin2].
+        apply in_dtree_dom__is_dtree_walk in Hin1.
+        apply in_dtrees_dom__is_dtree_walk in Hin2.
+        destruct Hdisj as [Hnotin _].
+        destruct Hin2 as [dt [Hinchs Hwk2]].
+        assert (idom p (get_dtree_root dt)) as Hsdom2.
+          eapply forall_parent_children__in_children; eauto.
+        eapply dtree_walk__clos_refl_trans_idom in Hin1; eauto.
+        assert (dtree_is_sound Hdec dt idom) as Hsd2.
+          apply DT_cons_is_sound_inv in Hp.
+          destruct Hp as [Hp1' Hp2'].
+          eapply dtrees_is_sound__dtree_is_sound; eauto.
+        eapply dtree_walk__clos_refl_trans_idom in Hwk2; eauto.
+        assert (get_dtree_root d <> get_dtree_root dt) as Hneq.
+          eapply notin_get_dtrees_roots__neq; eauto.
+        assert (sdom (get_dtree_root d) (get_dtree_root dt) \/
+                sdom (get_dtree_root dt) (get_dtree_root d)) as Hdec0.
+          eapply TCfg.rt_idom__sdom_ordered; 
+            eauto using inter_reachable_dtree_is_reachable.
+        eapply TCfg.idom_injective in Hdec0; 
+          eauto using reachable_dtrees__reachable_root,
+                      reachable_dtree__reachable_root.
+Qed.
+
+Lemma create_dtree__wf_dtree: forall (dt:DTree) 
+  (Hp: dtree_is_sound Hdec dt idom) (Hdj: disjoint_children_dtree Hdec dt)
+  (Hrd: reachable_dtree dt), 
+  wf_dtree dt.
+Proof.
+  intros.
+  destruct create_dtree__wf_dtree_mutrec as [J1 J2].
+  unfold create_dtree__wf_dtree_prop in J1; auto.
+Qed.
+
+Definition wf_dtree__uniq_dtree_prop (dt:DTree) :=
+  forall (Hp: wf_dtree dt), uniq_dtree Hdec dt.
+
+Definition wf_dtree__uniq_dtrees_prop (dts:DTrees) :=
+  forall (Hp: wf_dtrees dts), uniq_dtrees Hdec dts.
+
+Lemma wf_dtree__uniq_dtree_mutrec :
+  (forall dt, wf_dtree__uniq_dtree_prop dt) *
+  (forall dts, wf_dtree__uniq_dtrees_prop dts).
+Proof.
+  apply dtree_mutrec;
+    unfold wf_dtree__uniq_dtree_prop, wf_dtree__uniq_dtrees_prop;
+    simpl; intros; inv Hp; constructor; auto.
+Qed.
+
+Lemma wf_dtree__wf_dtree: forall (dt:DTree) (Hp: wf_dtree dt),
+  uniq_dtree Hdec dt.
+Proof.
+  intros.
+  destruct wf_dtree__uniq_dtree_mutrec as [J1 J2].
+  unfold wf_dtree__uniq_dtree_prop in J1; auto.
+Qed.
+
+End create_dtree__wf_dtree.
+
+End DTreeProps.
